riscv_model/spec/rsa_ops.dfy
@@ -1,0 +1,40 @@
+include "rv_consts.dfy"
+include "bv_ops.dfy"
+include "rv_ops.dfy"
+include "../lib/powers.dfy"
+include "../lib/congruences.dfy"
+
+module rsa_ops {
+    import opened rv_consts
+    import opened bv_ops
+    import opened rv_ops
+    import opened powers
+    import opened congruences
+
+    /* to_nat definions & lemmas */
+
+    function {:opaque} to_nat(xs: seq<uint32>): nat
+    {
+        if |xs| == 0 then 0
+        else
+            var len' := |xs| - 1;
+            to_nat(xs[..len']) + xs[len'] * pow_B32(len')
+    }
+
+    lemma to_nat_lemma_0(xs: seq<uint32>)
+        requires |xs| == 1
+        ensures to_nat(xs) == xs[0]
+    {
+        reveal to_nat();
+        reveal power();
+    }
+
+    lemma to_nat_lemma_1(xs: seq<uint32>)
+        requires |xs| == 2
+        ensures to_nat(xs) == xs[0] + xs[1] * BASE_32
+    {
+        reveal to_nat();
+        to_nat_lemma_0(xs[..1]);
+        reveal power();
+    }
+}
